\chapter{Limits}

\begin{problem}
	\enum{
	\item Let $f(x)=x^2-1$ and $g(x)=\frac{1}{x+1}$, we get $\lim_{x\to 1}f(x)=0$ and $\lim_{x\to1}g(x)=\frac{1}{2}$. Then we get $$\lim_{x\to 1}(f\cdot g)(x)=0.$$
	
	\item Expanding $x^3-2^3$ and noting that $x\neq 2$
	\begin{gather*}
		\lim_{x\to 2}\frac{(x-2)(x^2+2x+4)}{x-2}=\lim_{x\to 2}x^2+2x+4=12.
	\end{gather*}

	\item Expanding using 
	$$x^n-y^n=(x-y)(x^{n-1}+x^{n-2}y+\cdots +xy^{n-2}+y^{n-1})$$
	we get
	$$\lim_{x\to y}(x^{n-1}+x^{n-2}y+\cdots +xy^{n-2}+y^{n-1}) = y^n.$$
	
	\item Same thing here except we get $x^n$.
	
	\item Expand the fraction by the conjugate of the numerator
	\begin{align*}
		\lim_{h\to 0}\frac{\sqrt{a+h}-\sqrt{a}}{h}&=\lim_{h\to 0}\frac{h}{h(\sqrt{a+h}+\sqrt{a})} \\
		\lim_{h\to 0}\frac{1}{\sqrt{a+h}+\sqrt{a}}&=\frac{1}{2\sqrt{a}}
	\end{align*}
	}
\end{problem}