\chapter{Basic Properties of Numbers}

\begin{problem} ~\\ % 1
	\enum{
	\item Suppose that $ax=a$ and $a\neq 0$, then there exists a number $a^{-1}$. Multiplying $a^{-1}$ on both sides yields
		\begin{align*}
			(a^{-1}a) \cdot x &=a^{-1}a \\
			x &=1
		\end{align*}
	as desired.
	
	\item We use the distributive property on $(x-y)(x+y)$, this can be done by letting $a=x-y$: 
	\begin{align*}
		&(x-y)(x+y) = a(x+y)\\
		&=ax+ay = (x-y)x+(x-y)y\\
		&=x^2-yx+xy-y^2=x^2-y^2
	\end{align*}

	\item If we have $x^2=y^2$ then we certainly have $x^2-y^2=0$. By (ii) we know that $0=(x-y)(x+y)$, this implies that $x-y=0$ or $x+y=0$, this is equivalent to saying that $x=y$ or $x=-y$.

	\item Same method as (ii):
	\begin{align*}
		&a(x^2+xy+y^2) = ax^2+axy+ay^2\\
		&= (x-y)x^2+(x-y)xy+(x-y)y^2\\
		&=x^3-yx^2+x^2y-xy^2+xy^2-y^3\\
		&=x^3-y^3
	\end{align*}

	\item We prove this by induction, the base case $n=2$ is already proven in (ii). Suppose $x^n-y^n=(x-y)(x^{n-1}+x^{n-2}y+\cdots +xy^{n-2}+y^{n-1})$ is true. Then we equivalently have $x^n=(x-y)(x^{n-1}+x^{n-2}y+\cdots +xy^{n-2}+y^{n-1})+y^n$. We now prove the n+1 case:
	\begin{align*}
		&x^{n+1}-y^{n+1}=x\cdot x^n-y^{n+1} \\
		&=x(x-y)(x^{n-1}+x^{n-2}y+\cdots +xy^{n-2}+y^{n-1})+xy^n-y^{n+1} \\
		&=(x-y)(x^{n}+x^{n-1}y+\cdots +x^2y^{n-2}+xy^{n-1})+(x-y)y^n \\
		&=(x-y)(x^{n}+x^{n-1}y+\cdots +xy^{n-1}+y^n)
	\end{align*}
		The resulting relation concludes the finite induction, thus $x^n-y^n=(x-y)(x^{n-1}+x^{n-2}y+\cdots +xy^{n-2}+y^{n-1})$.
		
	\item We know from (iv) that $a^3-b^3=(a-b)(a^2+ab+b^2)$, by letting $a=x$ and $b=-y$ we get $x^3+y^3=(x+y)(x^2-xy+y^2)$.
 	}
\end{problem}

\begin{problem} % 2
	Multiplying by the multiplicative inverse of $x-y$ works only when $x-y\neq 0$, that is $x\neq y$, however, the hypothesis explicitly states $x=y$. So it is not possible to find the multiplicative inverse of $x-y$ and thus the step is invalid.
\end{problem}


\begin{problem} ~\\ % 3
	\enum{
	\item Say we have $\frac{a}{b}$ and $b\neq 0$ then the same fraction can be written as $ab^{-1}$. Suppose we also have a variable $c$ such that $c \neq 0$, then we have $ab^{-1} \cdot (cc^{-1})$ and consequently $(ac)(b^{-1}c^{-1})=\frac{ac}{bc}$. The final equality holds by (iii) which is proven below.
	
	\item By (i) $\frac{ad}{bd}+\frac{bc}{db} = ad(bd)^{-1}+bc(bd)^{-1}=(ad+bc)(bd)^{-1}=\frac{ad+bc}{bd}$
	
	\item $ab$ exists if $a,b \neq 0$. Let $x=(ab)^{-1}$, then
	\begin{align*}
		&x(ab)=(ab)^{-1}(ab) = (xa)b = 1 \hspace{1cm} &\texttt{(Multiply $x$ with $ab$)}\\
		&(xa)(bb^{-1})=b^{-1}=xa=b^{-1} &\texttt{(Multiply by $b^{-1})$} \\
		&x(aa^{-1})=b^{-1}a^{-1} = x& \texttt{(Multiply by $a^{-1}$)}
	\end{align*}
	
	\item Suppose $b,d\neq 0$, then $\frac{a}{b} \cdot \frac{c}{d}=(ab^{-1}) \cdot (cd^{-1}) =(ac)(b^{-1}d^{-1})=(ac)(bd)^{-1}=\frac{ac}{bd}$

	\item Suppose $b,c,d \neq 0$, then $\frac{a}{b} \big/ \frac{c}{d}=(ab^{-1})(cd^{-1})^{-1}=(ab^{-1})(c^{-1}d)=(ac)(bd)^{-1}=\frac{ac}{bd}$
	
	\item Suppose $b,d \neq 0$. Assume $\frac{a}{b}=\frac{c}{d}$, multiplying by $bd$ on both side yields the relation $ad=bc$. For the converse multiply $ad=bc$ by $(bd)^{-1}$.
	}
\end{problem}

\begin{problem} ~\\
	\enum{
	\item $4-x < 3-2x \iff (4-4)+(-x+2x) < (3-4)+(2x-2x) \iff x < -1$.
	
	\item $5-x^2<8 \iff -3 < x^2$. Note that $x^2 \geq 0$ and for every single value of $x$, so our solution is every $x$.
	
	\item $5-x^2 < -2 \iff 7 < x^2 \iff \sqrt{7} < x$ or $-\sqrt{7} > x $.

	\item The product is positive when $x-1 > 0$ and $x-3>0$ or when $x-1 < 0$ and $x-3<0$, that is when $x > 3$ or when $x<1$.
	
	\item Complete the square $x^2-2x+2=(x-1)^2+1$. The product $(x-1)^2$ is always positive, and since we have the $+1$ as well in the inequality, this inequality must be true for every single $x$.
	
	\item The inequality is equivalent to $x^2+x-1 > 0$. Completing the square $(x+\frac{1}{2})^2 > \frac{5}{4}$. If $x \geq -\frac{1}{2}$ then $x > \frac{-1+\sqrt{5}}{2}$. If $x < -\frac{1}{2}$ then $x < \frac{-1-\sqrt{5}}{2}$. Thus, the solution is $x > \frac{-1+\sqrt{5}}{2}$ and $x <\frac{-1-\sqrt{5}}{2}$.
	
	\item Equivalently we have $(x-\frac{1}{2})^2>\frac{25}{4}$. If $x\geq \frac{1}{2}$ then $x > 3$ if $x < \frac{1}{2}$ then $x < -2$. The solution set is $x >3$ and $x <-2$.
	
	\item Equivalently $(x+\frac{1}{2})^2+\frac{3}{4} > 0$. This is true for every x because $(x+\frac{1}{2}) \geq$ and $\frac{3}{4}> 0$. Adding them gives $(x+\frac{1}{2})^2 +\frac{3}{4} > 0$.
	
	\item Let $b=(x+5)(x-3)$. Then $b$ is positive if $x > 3$ or $x < -5$ and negative if $-5<x<3$. Let $a=x-\pi$. $a$ is positive if $x > \pi$. $ab$ is positive if both $a$ and $b$ are positive or if both are negative. So $ab$ is positive if $x > \pi$ ($b$ must be positive because $x > 3$). $ab$ is negative if $-5<x<3$ (This implies $x<\pi$).
	
	\item If $x > \sqrt[3]{2}$ and $x > \sqrt{2}$ then the product is positive, thus the first solution is $x > \sqrt{2}$. If $x < \sqrt[3]{2}$ and $x < \sqrt{2}$ then the product is positive. The second solution is $x < \sqrt[3]{2}$.
	
	\item Apply $\log_2$ on both sides: $x < 3$.
	
	\item Suppose $x < 1$, we will show this is a solution. We have $3^x<3^1 = 3$, adding $x<1$ to the inequality we get $x+3^x<3+1=4$. Since both $3^x$ and $x$ are strictly increasing expressions finding the inequality $x<1$ suffices as all real solutions.
	
	\item Noting that $x\neq 0$ and $x\neq 1$. Expanding the fractions we get $\frac{1-x}{x(1-x))}+\frac{x}{x(1-x)}=\frac{1}{x(1-x)}>0$. The solutions depends on if the denominator is positive. Thus $x(1-x)>0$ has the same solution set. The solutions are $0 < x < 1$.
	
	\item Note $x\neq -1$. Expand by $(x+1)$: $\frac{(x-1)(x+1)}{(x+1)^2}>0$. Since the denominator is always positive we can multiply this on both sides, $x^2-1>0$, Thus $x < -1$ and $x > 1$.
	}
\end{problem}

\begin{problem} ~\\
	\enum{
	\item Suppose $a<b$ and $c<d$ then we have $b-a>0$ and $d-c >0$ by property 11 $(b-a)+(d-c) > 0$ which is the same as $b+d>a+c$.
	
	\item Suppose $a < b$ then $0 < b-a \iff -b < (b-b)-a = -b < -a$.
	
	\item Suppose $a < b$ and $c < d$, by (ii): $-c < -d$, then by (i) we have $a-d < b-d$.
	
	\item Suppose $a < b$ then $b-a > 0$. Assume $c>0$, Using (P12) we know that $c(b-a) > 0$ and consequently $bc-ac > 0 \iff bc > ac$.
	
	\item Suppose $a < b$ then $b-a > 0$. Assume $c<0$, then by (ii) we have $-c>0$. Using P12 we know that $-c(b-a) > 0$ and consequently $ac-bc > 0 \iff ac > bc$.
	
	\item Since $a > 1 > 0$ we apply (iv) by letting $c=a$. Thus $a^2>a$.
	
	\item Because $a$ is positive, it follows by applying (iv) to $a < 1$ that $a^2 <a$.
	
	\item Using (iv), multiply $a<b$ with $c$ and $c<d$ with $b$. This means that we have $ac<bc$ and $bc<bd$, this is the same as $ac<bc<bd$, thus $ac <bd$.
	
	\item Using (viii) we multiply the same inequality twice, $a^2<b^2$.
	
	\item Suppose $a,b\geq 0$, we prove the contra-positive, therefore $a\geq b$. Multiply by $a$ and $b$ respectively gives two inequalities $a^2 \geq ab$ and $ab \geq b^2$ which is the same as $a^2\geq ab \geq b^2$. This concludes the contra-positive proof because $a^2 \geq b^2$ is the logical opposite of $a^2 < b^2$.
}
\end{problem}

\begin{problem} ~\\
	\enuma{
		\item The base case is $n=2$ which was proven in problem 1.5. Assume $x^n<y^n$ for $0 \leq x < y$. By problem 1.6. (viii) we have $x \cdot x^n < y \cdot y^n \iff x^{n+1}<y^{n+1}$. The induction is complete, thus if $0 \leq x,y$ then $x^n<y^n$ for $n=1,2,\ldots$.
		
		\item Suppose $x<y$ and $n=2k+1$, We have three cases.
		\enum{
			\item $x,y \geq 0$, this case has been proven in (a).
			\item $x \leq 0$ and $y \geq 0$. Consider $x^n$, because $n$ is odd, it has the following property, $x^{2k+1}=x \cdot (x^k)^2 < 0$, because $x$ is negative and $(x^k)^2$ is positive. However $y^n>0$ because $y$ is positive. This means we have $x^n<0<y^n$.
			
			\item $x,y < 0$, by the inequality we have $-x > 0$ and $-y > 0$. We also have $-y < -x$, by (a) we have $(-y)^n<(-x)^n \iff -y^n < -x^n$ because n is odd. Finally we have $x^n < y^n$.
		}
	
		\item Suppose $x^n=y^n \iff x^n-y^n=0 = (x-y)(x^{n-1}+x^{n-2}y+ \cdots + xy^{n-2}+y^{n-1})$ Then either $x-y=0$ or $x^{n-1}+x^{n-2}y+ \cdots + xy^{n-2}+y^{n-1}=0$ In the first case $x=y$, in the second case we first note that $x^n=y^n$ implies that $x$ and $y$ has the same sign and thus $x^{n-1}+x^{n-2}y+ \cdots + xy^{n-2}+y^{n-1} \geq 0$ where the equality holds only when $x,y=0$ then $x=y$ is still true. 
		
		\item Let $n$ be an even positive integer. Next we prove the contra-positive, suppose $|x| \neq |y|$ ($x=y$ or $x=-y$ is the same as saying $|x|=|y|$). Consequently this means either $|x|<|y|$ or $|x|>|y|$. By (a) this means that either $|x|^n<|y|^n$ or $|x|^n>|y|^n$. Because $n$ is even this is equivalent to $x^n<y^n$ or $x^n>y^n$ which is the logical complement of $x^n=y^n$.
	}
\end{problem}

\begin{problem}
	Suppose $0<a<b$, multiply by $a$ then $a^2<ab \iff a < \sqrt{ab}$. Next consider $(a-b)^2 > 0$ which is equivalent to $a^2+b^2 +2ab > 4ab \iff \frac{a+b}{2} > \sqrt{ab}$, this means that we have $a<\sqrt{ab}<\frac{a+b}{2}$ now remains the final inequality. By the premise we have $b-a>0 \iff b+a>2a \iff \frac{b+a}{2}>a$. We conclude by stating $a<\sqrt{ab}<\frac{a+b}{2}<b$.
\end{problem}

\begin{*problem} ~\\
	\begin{itemize}
		\item [(P10)] Let $b=0$ in P'10, then for every $a$ one of the following properties apply 
		\enum{
			\item $a=0$
			\item $a<0$
			\item $a>0$
		}
		Because the collection $P$ contains all the numbers $x$ such that $x>0$, we can see that (iii) states that $a$ belongs to $P$. (ii) is equivalent to $-a>0$, thus -a is  in $P$.
		\item [(P11)] Suppose $x$ and $y$ are in $P$ then $0<x$ and $0<y$. By P'12 (Let a=0) we have $x<y+x$. By P'11  we get $0<y+x$ which is in $P$.
		\item [(P12)] Suppose $x$ and $y$ are in $P$ then $0<x$ and $0<y$. Using P'13 we get $0<xy$, this means that $xy$ is in $P$.
	\end{itemize}
\end{*problem}

\begin{problem}
	\enum{
	\item $\sqrt{2}+\sqrt{3}-\sqrt{5}+\sqrt{7}$.
	\item Triangle inequality states that $|a+b|-|a|-|b|\leq 0$. Therefore $|a|+|b|-|a+b|$.
	\item Triangle inequality gives $|(a+b)+c| -|a+b|-|c| \leq 0 \iff |a+b|+|c|-|a+b+c|. \geq 0$. Our solution is therefore $|a+b|+|c|-|a+b+c|$.
	\item $x^2-2xy+y^2=(x-y)^2\geq 0$, thus $x^2-2xy+y^2$.
	\item $\sqrt{2}+\sqrt{3}+\sqrt{5}-\sqrt{7}$
	}
\end{problem}

\begin{problem}
	
\end{problem}